feat: loop constructor

CollapsingTowers/TwoLevelRec/CtxEquiv/ObsCtx.lean
@@ -121,11 +121,6 @@ lemma typing.congruence_under_ObsCtxℂ :
     apply IH; apply typing.congruence_under_ObsCtx𝔹
     apply Hτ; apply HB
 
--- e₁⇓ ≜ ∃ v, e ⇝* v
-@[simp]
-def termination (e : Expr) : Prop :=
-  ∃ v, value v ∧ e ⇝* v
-
 -- Γ ⊢ e₀ ≤𝑐𝑡𝑥 e₁ : τ ≜
 --   Γ ⊢ e₀ : τ ∧
 --   Γ ⊢ e₁ : τ ∧
