CollapsingTowers/TwoLevelRec/OperationalSemantics/Confluence.lean
@@ -114,3 +114,18 @@ theorem stepn.unique_normal_forms :
   have HEq₀ := stepn.value_impl_termination _ _ Hvalue₀ Hstep₀
   have HEq₁ := stepn.value_impl_termination _ _ Hvalue₁ Hstep₁
   rw [HEq₀, HEq₁]
+
+theorem stepn_indexed.unique_normal_forms :
+  ∀ il ir e v₀ v₁,
+    (e ⇝ ⟦il⟧ v₀) →
+    (e ⇝ ⟦ir⟧ v₁) →
+    value v₀ →
+    value v₁ →
+    v₀ = v₁ ∧ il = ir :=
+  by
+  intros il ir e v₀ v₁ Hstep₀ Hstep₁ Hvalue₀ Hvalue₁
+  have ⟨z₀, z₁, r, HEq, Hstep₀, Hstep₁⟩ := stepn_indexed.church_rosser _ _ _ _ _ Hstep₀ Hstep₁
+  have ⟨HEqv₀, HEqz₀⟩:= stepn_indexed.value_impl_termination _ _ _ Hvalue₀ Hstep₀
+  have ⟨HEqv₁, HEqz₁⟩:= stepn_indexed.value_impl_termination _ _ _ Hvalue₁ Hstep₁
+  simp [HEqv₀, HEqv₁]
+  omega
