CollapsingTowers/TwoLevelRec/OperationalSemantics/Defs.lean
@@ -5,3 +5,4 @@ import CollapsingTowers.TwoLevelRec.OperationalSemantics.Congruence
 import CollapsingTowers.TwoLevelRec.OperationalSemantics.Deterministic
 import CollapsingTowers.TwoLevelRec.OperationalSemantics.Confluence
 import CollapsingTowers.TwoLevelRec.OperationalSemantics.Refine
+import CollapsingTowers.TwoLevelRec.OperationalSemantics.Termination
