CollapsingTowers/TwoLevelRec/OperationalSemantics/Termination.lean
@@ -1,0 +1,85 @@
+import CollapsingTowers.TwoLevelRec.OperationalSemantics.Refine
+
+-- e₁⇓ ≜ ∃ v, e ⇝* v
+@[simp]
+def termination (e : Expr) : Prop :=
+  ∃ v, value v ∧ e ⇝* v
+
+-- λf.λx.f @ x
+@[simp]
+def fᵥ : Expr := .lam (.lam (.app₁ (.bvar 1) (.bvar 0)))
+
+-- (λy.fᵥ @ fix(fᵥ) @ y) @ 17
+@[simp]
+def loop₀ : Expr := .app₁ (.lam (.app₁ (.app₁ fᵥ (.fix₁ fᵥ)) (.bvar 0))) (.lit 17)
+
+-- fᵥ @ fix(fᵥ) @ 17
+@[simp]
+def loop₁ : Expr := .app₁ (.app₁ fᵥ (.fix₁ fᵥ)) (.lit 17)
+
+-- fᵥ @ (λy.fᵥ @ fix(fᵥ) @ y) @ 17
+@[simp]
+def loop₂ : Expr := .app₁ (.app₁ fᵥ (.lam (.app₁ (.app₁ fᵥ (.fix₁ fᵥ)) (.bvar 0)))) (.lit 17)
+
+-- (λx.(λy.fᵥ @ fix(fᵥ) @ y) @ x) @ 17
+@[simp]
+def loop₃ : Expr := .app₁ (.lam (.app₁ (.lam (.app₁ (.app₁ fᵥ (.fix₁ fᵥ)) (.bvar 0))) (.bvar 0))) (.lit 17)
+
+@[simp]
+def step₀ : (loop₀ ⇝ loop₁) :=
+  by
+  simp
+  apply step_lvl.pure id
+  apply ctx𝕄.hole
+  repeat constructor
+
+@[simp]
+def step₁ : (loop₁ ⇝ loop₂) :=
+  by
+  simp
+  apply step_lvl.pure (fun X => .app₁ (.app₁ fᵥ X) (.lit 17))
+  apply ctx𝕄.cons𝔹 _ _ (ctx𝔹.appl₁ _ _)
+  apply ctx𝕄.cons𝔹 _ _ (ctx𝔹.appr₁ _ _)
+  apply ctx𝕄.hole
+  repeat constructor
+
+@[simp]
+def step₂ : (loop₂ ⇝ loop₃) :=
+  by
+  simp
+  apply step_lvl.pure (fun X => .app₁ X (.lit 17))
+  apply ctx𝕄.cons𝔹 _ _ (ctx𝔹.appl₁ _ _)
+  apply ctx𝕄.hole
+  repeat constructor
+
+@[simp]
+def step₃ : (loop₃ ⇝ loop₀) :=
+  by
+  simp
+  apply step_lvl.pure id
+  apply ctx𝕄.hole
+  repeat constructor
+
+lemma termination.loop_impl_refl : ∀ z e, (e ⇝ ⟦z⟧ e) → termination e → z = 0 :=
+  by
+  intros zl₀ e Hstepl₀ Htermination
+  have ⟨v, Hvalue, Hstepr₀⟩ := Htermination
+  have ⟨zr₀, Hstepr₀⟩ := stepn_impl_stepn_indexed _ _ Hstepr₀
+  have ⟨zl₁, zr₁, r, HEq, Hstepl₁, Hstepr₁⟩ := stepn_indexed.church_rosser _ _ _ _ _ Hstepl₀ Hstepr₀
+  have ⟨HEqv, HEqzr₁⟩:= stepn_indexed.value_impl_termination _ _ _ Hvalue Hstepr₁
+  rw [← HEqv] at Hstepl₁
+  have ⟨_, HEqz⟩ := stepn_indexed.unique_normal_forms _ _ _ _ _ Hstepr₀ Hstepl₁ Hvalue Hvalue
+  omega
+
+theorem termination.loop : ¬termination loop₀ :=
+  by
+  intro Htermination
+  have Hstep : (loop₀ ⇝ ⟦4⟧ loop₀) :=
+    by
+    apply stepn_indexed.multi _ _ _ _ step₀
+    apply stepn_indexed.multi _ _ _ _ step₁
+    apply stepn_indexed.multi _ _ _ _ step₂
+    apply stepn_indexed.multi _ _ _ _ step₃
+    apply stepn_indexed.refl
+  have H := termination.loop_impl_refl _ _ Hstep Htermination
+  omega
